update NextSendVoteStepSendFunc to also take v' as argument

messageInvariantPrototypes/twoPhaseCommit/decentralizedMonotonic/distributedSystem.dfy
@@ -103,6 +103,10 @@ module DistributedSystem {
     ghost predicate ValidHistoryIdx(i: int) {
       0 <= i < |history|
     }
+    
+    ghost predicate ValidHistoryIdxStrict(i: int) {
+      0 <= i < |history|-1
+    }
 
     ghost predicate WF(c: Constants) {
       && c.WF()
